cogent/llvm/checker/coq/Correctness.v
@@ -7,22 +7,18 @@ From Vellvm Require Import LLVMAst LLVMEvents TopLevel Handlers InterpreterMCFG 
   DynamicValues ExpLemmas Coqlib NoFailure AListFacts.
 
 From Checker Require Import Denotation DenotationTheory Cogent Compiler Utils.Tactics Invariants
-  HelixLib.Correctness_Prelude HelixLib.BidBound.
+  HelixLib.Correctness_Prelude HelixLib.BidBound HelixLib.IdLemmas.
 
 Import ListNotations.
 Import RecordSetNotations.
 Import AlistNotations.
 
-Definition vellvm_prog : Type := toplevel_entities typ (LLVMAst.block typ * list (LLVMAst.block typ)).
-Definition ocfg_res : Type := (block_id * block_id) + uvalue.
-
-Definition semantics_cogent (p : cogent_prog) : failT (itree E_mcfg) (memoryC * uval) := 
-  interp_cogent (denote_program p) "main" UUnit empty_memory.
-
 Import ExpTactics.
 Import ProofMode.
 
 Section Expressions.
+
+  Definition ocfg_res : Type := (block_id * block_id) + uvalue. 
 
   (* From Helix *)
   Definition branches (to : block_id) : Rel_cfg_T uval ocfg_res :=
@@ -37,19 +33,19 @@ Section Expressions.
 
   Lemma compile_expr_correct :
     forall (e : expr) (γ : ctx) (s1 s2 : IRState)
-           (v : im) (nextblock bid_in bid_from : block_id) (bks : ocfg typ)
+           (v : im) (next_bid entry_bid prev_bid : block_id) (blks : ocfg typ)
            (memC : memoryC) (g : global_env) (l : local_env) (memV : memoryV),
-      compile_expr e nextblock s1 ≡ inr (s2, (v, bid_in, bks)) ->
+      compile_expr e next_bid s1 ≡ inr (s2, (v, entry_bid, blks)) ->
       no_failure (interp_expr (E := E_cfg) (denote_expr γ e) memC) ->
-      bid_bound s1 nextblock ->
+      bid_bound s1 next_bid ->
       state_invariant γ s1 memC (memV, (l, g)) ->
       eutt
-        (succ_cfg (compile_expr_post v γ s1 s2 nextblock l))
+        (succ_cfg (compile_expr_post v γ s1 s2 next_bid l))
         (interp_expr (denote_expr γ e) memC)
-        (interp_cfg (denote_ocfg (convert_typ [] bks) (bid_from,bid_in)) g l memV).
+        (interp_cfg (denote_ocfg (convert_typ [] blks) (prev_bid, entry_bid)) g l memV).
   Proof.
     induction e; intros * COMPILE NOFAIL NEXT PRE.
-    - (* compile_expr Unit *)
+    - (* Unit *)
       cbn* in *; simp.
       cbn*.
       rewrite denote_ocfg_unfold_not_in.
@@ -61,7 +57,7 @@ Section Expressions.
       go; reflexivity.
       apply local_scope_modif_refl.
       apply find_block_nil.
-    - (* compile_expr (Lit l) *)
+    - (* Lit l *)
       cbn* in *; simp.
       cbn*.
       rewrite denote_ocfg_unfold_not_in.
@@ -74,7 +70,7 @@ Section Expressions.
         go; reflexivity.
       apply local_scope_modif_refl.
       apply find_block_nil.
-    - (* compile_expr (LVar i) *)
+    - (* LVar i *)
       cbn* in *; simp.
       rewrite denote_ocfg_unfold_not_in.
       cvred.
@@ -94,22 +90,71 @@ Section Expressions.
       apply failure_expr_throw in NOFAIL.
       contradiction.
       apply find_block_nil.
-    (* -
-      cbn* in COMPILE; simp.
-      unfold denote_expr, option_bind in *; cbn*; simp.
-      2 : apply failure_expr_throw in NOFAIL; contradiction.
-      rewrite interp_expr_Ret.
-      rewrite denote_code_nil.
-      vred.
-      apply eutt_Ret; split; [ | split]; cbn; eauto.
-      intros.
-      unfold id in *; cbn* in *.
-      destruct PRE as [MEM WF]; unfold memory_invariant in MEM.
-      specialize (MEM _ _ _ Heqo0 Heqo).
-      unfold equivalent_values in MEM.
-      specialize (MEM l' H H0).
+    - (* Let e1 e2 *)
+      pose proof COMPILE as COMPILE'.
+      cbn* in COMPILE'; simp.
+      rename s1 into pre_state, i into mid_state, i1 into post_state.
+      rename Heqs into COMPILE_e1, Heqs1 into COMPILE_e2.
+      
+      specialize (IHe1 γ _ _ _ _ _ entry_bid _ memC g l memV COMPILE_e1).
+      forward IHe1.
+      eapply no_failure_expr_bind_prefix; exact NOFAIL.
+      forward IHe1.
+      (* don't like manual instantiation here *)
+      apply bid_bound_incBlockNamed with (name := "Let") (s1 := pre_state).
+      solve_prefix.
+      reflexivity.
+      forward IHe1.
+      apply state_invariant_new_block. (* unproven lemma *)
       assumption.
-    -
+      
+      rewrite convert_typ_ocfg_app.
+      rewrite denote_ocfg_app.
+      (* 2 : {
+        idtac.
+        unfold no_reentrance.
+        rewrite convert_typ_outputs, inputs_convert_typ, outputs_cons.
+        unfold successors, terminator_outputs, blk_term.
+        simpl.
+        apply list_disjoint_cons_l.
+        admit.
+      } *)
+      admit.
+      admit.
+    - (*BPrim op e1 e2*)
+      cbn* in *; simp.
+      admit.
+    - (*If e1 e2 e3 *)
+      admit.
+    (*
+    - 
+      cbn* in *; simp.
+      rename s1 into pre_state, c0 into mid_state, s2 into post_state.
+      rename Heqs into COMPILE_e1, Heqs0 into COMPILE_e2.
+      vred.
+
+      specialize (IHe1 γ _ _ _ _ cogent_mem g l vellvm_mem COMPILE_e1).
+      forward IHe1; auto.
+      forward IHe1.
+      eapply no_failure_expr_bind_prefix; exact NOFAIL.
+      rewrite interp_expr_bind.
+
+      (* might not need the following 3 *)
+      eapply eutt_clo_bind_returns ; [eassumption | clear IHe1].
+      introR; destruct_unit.
+      intros RET1 _; eapply no_failure_expr_bind_continuation in NOFAIL; [| eassumption]; clear RET1.
+      cbn in PRE0.
+      destruct PRE0 as (PRE1 & [EXP1]).
+      cbn in *.
+
+      specialize (IHe2 (vC :: γ) _ _ _ _ memC g0 l0 memV COMPILE_e2).
+      forward IHe2.
+      apply state_invariant_new_var; auto.
+      unfold equivalent_values.
+      intros.
+      specialize (EXP1 l'). 
+      
+     -
       cbn* in *; simp.
       rename s1 into pre_state, c0 into mid_state, c2 into post_state.
       rename e0 into res_e1, e3 into res_e2, c1 into code_e1, c3 into code_e2.
@@ -155,77 +200,17 @@ Section Expressions.
         admit.
       }
       admit.
-    -
-      cbn* in COMPILE; simp.
-      unfold denote_expr in *; cbn*.
-      rewrite interp_expr_Ret.
-      rewrite denote_code_nil.
-      vred.
-      apply eutt_Ret; split; [ | split]; cbn; eauto.
-      intros.
-      typ_to_dtyp_simplify.
-      unfold denote_exp; cbn.
-      go; reflexivity.
-    -
-      cbn* in COMPILE; simp.
-      unfold denote_expr in *; cbn*.
-      rewrite interp_expr_Ret.
-      rewrite denote_code_nil.
-      vred.
-      apply eutt_Ret; split; [ | split]; cbn; eauto.
-      intros.
-      destruct l;
-        simpl;
-        typ_to_dtyp_simplify;
-        unfold denote_exp; cbn;
-        go; reflexivity.
-    - 
-      cbn* in *; simp.
-      rename s1 into pre_state, c0 into mid_state, s2 into post_state.
-      rename Heqs into COMPILE_e1, Heqs0 into COMPILE_e2.
-      vred.
-
-      specialize (IHe1 γ _ _ _ _ cogent_mem g l vellvm_mem COMPILE_e1).
-      forward IHe1; auto.
-      forward IHe1.
-      eapply no_failure_expr_bind_prefix; exact NOFAIL.
-      rewrite interp_expr_bind.
-
-      (* might not need the following 3 *)
-      eapply eutt_clo_bind_returns ; [eassumption | clear IHe1].
-      introR; destruct_unit.
-      intros RET1 _; eapply no_failure_expr_bind_continuation in NOFAIL; [| eassumption]; clear RET1.
-      cbn in PRE0.
-      destruct PRE0 as (PRE1 & [EXP1]).
-      cbn in *.
-
-      specialize (IHe2 (vC :: γ) _ _ _ _ memC g0 l0 memV COMPILE_e2).
-      forward IHe2.
-      apply state_invariant_new_var; auto.
-      unfold equivalent_values.
-      intros.
-      specialize (EXP1 l'). *)
-      
-      
-      
-      
-      
-      
-      
-      
-      
-
-      
-
-      
-
-      
+      *)
       
   Admitted.
 
 End Expressions.
 
 Section TopLevel.
+
+  Definition vellvm_prog : Type := toplevel_entities typ (LLVMAst.block typ * list (LLVMAst.block typ)).
+  Definition semantics_cogent (p : cogent_prog) : failT (itree E_mcfg) (memoryC * uval) := 
+    interp_cogent (denote_program p) "main" UUnit empty_memory.
 
   (* placeholder *)
   Definition TT {A B} (x: A) (y: B):= True.
